Instantiate loc_unused_in_not_unused_in_disjoint

ulib/LowStar.Modifies.fst
@@ -282,6 +282,9 @@ let loc_not_unused_in = MG.loc_not_unused_in _
 
 let loc_unused_in = MG.loc_unused_in _
 
+let loc_unused_in_not_unused_in_disjoint =
+  MG.loc_unused_in_not_unused_in_disjoint cls
+
 let live_loc_not_unused_in #t b h =
   B.unused_in_equiv b h;
   Classical.move_requires (MG.does_not_contain_addr_addr_unused_in h) (B.frameOf b, B.as_addr b);
